Verify

VRF/Hacl.VRF.Hash.fst
@@ -62,8 +62,8 @@ let _ECVRF_prove_2 proof secret =
 				let h3 = ST.get() in 
 				disjoint_sub_lemma2 bigNums (size 15) (size 5) (size 10) (size 5);
 			fdifference_reduced kf cxf; 
+			copy (size 16) clow chigh;	
 			fcontract s kf;
-			copy (size 16) chigh clow;	
 			true
 		)
 
@@ -117,73 +117,6 @@ let _ECVRF_prove #len proof inputLength input secret pk =
 	in 
 		if  not r then false else  
 			_ECVRF_prove_2 proof secret
-
-(*)
-val proofToHash:
-			beta: lbuffer uint8 (v size_hash) ->
-			gamma: point -> 
-			c: scalar -> s: scalar -> 
-			proof: lbuffer uint8 (v(size 80)) -> 	
-			Stacl bool
-		(requires  (fun h0 -> live h0 proof /\ live h0 gamma /\ live h0 beta))
-		(ensures (fun h0 _ h1 -> preserves_live h0 h1))
-			
-let proofToHash gamma proof = 
-	let r = decodeProof gamma c s proof in 
-	if not r then false else
-	let gamma' = sub proof (size 0) (size 32) in 
-	hash beta (size 32) gamma';
-	true
-
-
-val _ECVRF_verify:
-		points: lbuffer uint128 (v(size 160)) -> 
-		proof: lbuffer uint8 (v(size 80)) -> 
-		inputLength: size_t{v inputLength == len /\ uint_v inputLength < maxint SIZE - 97} -> 
-		input: lbuffer uint8 len -> 
-		Stack bool
-			(requires  (fun h0 -> live h0 proof /\ live h0 gamma /\ live h0 beta))
-			(ensures (fun h0 _ h1 -> preserves_live h0 h1))
-		
-let _ECVRF_verify pk proof inputLength input = 
-	let r = alloc #_ #(bool) (size 128) (u8(0)) 
-		[BufItem pk; BufItem proof; BufItem input] [] 
-		(fun h0 _ h1 -> True) 
-		(fun scalars ->
-	let pk = sub points (size 0) (size 20) in 
-	let yc = sub points (size 20) (size 20) in 
-	let g = sub points (size 40) (size 20) in 
-	let gs = sub points (size 60) (size 20) in 
-	let u = sub points (size 80) (size 20) in 
-	let gammac = sub points (size 100) (size 20) in 
-	let hs = sub points (size 120) (size 20) in 
-	let gamma = sub points (size 140) (size 20) in 		
-
-	let c = sub scalars (size 0) (size 32) in
-	let s = sub scalars (size 32) (size 32) in 
-	let h = sub scalars (size 64) (size 32) in 
-	let c_new = sub scalars(size 96) (size 32) in 
-	let c_small = sub c (size 0) (size 16) in 
-	let d = decodeProof gamma c_small s proof in 
-	if not d then false else
-	point_mult yc y c;
-	make_g g;
-	point_mult gs g s;
-	point_add u yc gs;
-	let r = _ECVRF_hash_to_curve h pk input in 
-	if not r then false else 
-	point_mult gammac gamma c;
-	point_mult hs h s;
-	point_add v gammac hs;
-	_ECVRF_hashPoints c_new h pk gamma u v;
-	c==c_new
-
-
-
-
-
-
-
 
 
 
