VRF/Hacl.VRF.HashVerify.fst
@@ -1,0 +1,107 @@
+module Hacl.VRF.HashVerify
+
+open FStar.Mul
+
+open FStar.HyperStack
+open FStar.HyperStack.ST
+module ST = FStar.HyperStack.ST
+
+open Spec.Lib
+open Spec.Lib.IntSeq
+
+open Spec.Lib.IntTypes
+open Spec.Lib.IntBuf
+open Spec.Lib.IntBuf.Lemmas
+
+open Hacl.VRF.HashToCurveFinal
+open Hacl.VRF.HashPoints
+open Hacl.VRF.DecodeProof
+
+open Hacl.VRF.Lib
+
+#reset-options " --z3rlimit 100"
+
+
+val point_sum : pointTo0: point -> pointTo1: point -> pointTo2: point -> 
+	pointFrom0: point -> scalarFrom0: word ->   
+	pointFrom1: point -> scalarFrom1: word -> 
+	Stack unit 
+		(requires (fun h0 -> live h0 pointTo0 /\ live h0 pointTo1 /\ live h0 pointTo2 /\
+			live h0 pointFrom0 /\ live h0 pointFrom1 /\ live h0 scalarFrom0 /\ live h0 scalarFrom1
+			/\ disjoint pointTo0 pointFrom0 /\ disjoint pointTo1 pointFrom1/\ 
+			disjoint pointTo2 pointTo0 /\ disjoint pointTo2 pointTo1
+		))
+		(ensures (fun h0 _ h1 -> preserves_live h0 h1 /\ modifies3 pointTo0 pointTo1 pointTo2 h0 h1 ))
+
+
+let point_sum pointTo0 pointTo1 pointTo2 pointFrom0 scalarFrom0 pointFrom1 scalarFrom1 = 
+	point_mult pointTo0 pointFrom0 scalarFrom0;
+	point_mult pointTo1 pointFrom1 scalarFrom1;
+	point_add pointTo2 pointTo0 pointTo1
+
+val _ECVRF_verify: 
+	#len : size_nat -> 
+	proof: lbuffer uint8 80 -> 
+	inputLength: size_t{v inputLength == len /\ len < maxint SIZE - 96} -> 
+	input: lbuffer uint8 len -> 
+	pk: point -> 
+	Stack bool 
+		(requires (fun h0 -> live h0 proof /\ live h0 input /\ live h0 pk))
+		(ensures (fun h0 _ h1 -> preserves_live h0 h1))
+
+let _ECVRF_verify #len proof inputLength input pk = 
+	alloc #_ #(bool) #(200) (size 200) (u64(0)) 
+		[BufItem proof; BufItem input; BufItem pk] 
+		[]
+		(fun h0 _ h1 -> True)
+		(fun pointBuffer -> 
+			let pubKey = sub pointBuffer (size 40) (size 20) in 
+			copy (size 20) pk pubKey;
+			let r_ = alloc #_ #(bool) #(64) (size 64) (u8 (0)) 
+			[BufItem proof; BufItem input; BufItem pointBuffer]
+			[BufItem pointBuffer]
+			(fun h0 _ h1 -> True)
+			(fun cs -> 
+
+				let generator = sub #_ #(200) #(20) pointBuffer (size 0) (size 20) in 
+				let h = sub #_ #(200) #(20) pointBuffer (size 20) (size 20) in 
+				let pk = sub #_ #(200) #(20) pointBuffer (size 40) (size 20) in 
+				let gamma = sub #_ #(200) #(20) pointBuffer (size 60) (size 20) in 
+				let u = sub #_ #(200) #(20) pointBuffer (size 80) (size 20) in
+				let v = sub #_ #(200) #(20) pointBuffer (size 100) (size 20) in 
+				let bufferToHash = sub #_ #(200) #(120) pointBuffer  (size 0) (size 120) in 
+
+				let yc = sub #_ #(200) #(20) pointBuffer (size 120) (size 20) in 
+				let gs = sub #_ #(200) #(20) pointBuffer (size 140) (size 20) in 
+				let gammac = sub #_ #(200) #(20) pointBuffer (size 160) (size 20) in 
+				let hs = sub #_ #(200) #(20) pointBuffer (size 180) (size 20) in 
+
+				let gamma' = sub proof (size 0) (size 32) in 
+				let c = sub #_ #(80) #(16) proof (size 32) (size 16) in 
+				let s = sub proof (size 48) (size 32) in 
+				let r = decompress gamma gamma' in 
+
+				if not r then false else begin
+
+				let cExtended = sub	cs (size 0) (size 32) in 
+				let cToCheck = sub cs (size 32) (size 32) in 
+				let partOfExtended = sub cs (size 0) (size 16) in 
+
+				copy (size 16) c partOfExtended; 
+				make_g generator;
+				point_sum yc gs u pk cExtended generator s;
+
+				let r = _ECVRF_hash_to_curve h pk inputLength input in
+				if not r then false
+				else begin	
+				point_sum gammac hs v gamma cExtended h s;
+				_ECVRF_hashPoints cToCheck bufferToHash;
+				let cToCheckLow = sub cToCheck (size 16) (size 16) in 
+				let r = equalBuffer cToCheckLow c in 
+				r 
+				end
+				end	
+ 	
+			)
+		in r_
+	)
